cedar-lean/Cedar/Thm/Partial/Subst.lean
@@ -1,0 +1,121 @@
+/-
+ Copyright Cedar Contributors
+
+ Licensed under the Apache License, Version 2.0 (the "License");
+ you may not use this file except in compliance with the License.
+ You may obtain a copy of the License at
+
+      https://www.apache.org/licenses/LICENSE-2.0
+
+ Unless required by applicable law or agreed to in writing, software
+ distributed under the License is distributed on an "AS IS" BASIS,
+ WITHOUT WARRANTIES OR CONDITIONS OF ANY KIND, either express or implied.
+ See the License for the specific language governing permissions and
+ limitations under the License.
+-/
+
+import Cedar.Data.Map
+import Cedar.Partial.Expr
+import Cedar.Partial.Value
+import Cedar.Spec.Expr
+import Cedar.Thm.Data.List
+
+/-! ## Lemmas about `subst` operations -/
+
+namespace Cedar.Thm.Partial.Subst
+
+open Cedar.Data
+open Cedar.Partial (Unknown)
+
+/--
+  subst on a concrete expression is that expression
+-/
+theorem subst_concrete_expr (expr : Spec.Expr) (subsmap : Map Unknown Partial.Value) :
+  expr.asPartialExpr.subst subsmap = expr.asPartialExpr
+:= by
+  unfold Partial.Expr.subst Spec.Expr.asPartialExpr
+  cases expr
+  case lit | var => simp only
+  case unaryApp op x₁ | getAttr x₁ attr | hasAttr x₁ attr =>
+    simp only [Partial.Expr.unaryApp.injEq, Partial.Expr.getAttr.injEq, Partial.Expr.hasAttr.injEq, true_and, and_true]
+    exact subst_concrete_expr x₁ subsmap
+  case and x₁ x₂ | or x₁ x₂ | binaryApp op x₁ x₂ =>
+    simp only [Partial.Expr.and.injEq, Partial.Expr.or.injEq, Partial.Expr.binaryApp.injEq, true_and, and_true]
+    constructor
+    · exact subst_concrete_expr x₁ subsmap
+    · exact subst_concrete_expr x₂ subsmap
+  case ite x₁ x₂ x₃ =>
+    simp only [Partial.Expr.ite.injEq]
+    and_intros
+    · exact subst_concrete_expr x₁ subsmap
+    · exact subst_concrete_expr x₂ subsmap
+    · exact subst_concrete_expr x₃ subsmap
+  case set xs | call xfn xs =>
+    simp only [Partial.Expr.set.injEq, Partial.Expr.call.injEq, true_and, and_true]
+    simp only [List.map₁_eq_map, List.map_map]
+    apply List.map_congr
+    intro x _
+    exact subst_concrete_expr x subsmap
+  case record attrs =>
+    simp only [Partial.Expr.record.injEq, Partial.Expr.record.injEq, true_and, and_true]
+    simp only [List.map_attach₂_snd, List.map_map]
+    apply List.map_congr
+    intro (a, x) h₁
+    simp only [Function.comp_apply, Prod.mk.injEq, true_and]
+    have := List.sizeOf_snd_lt_sizeOf_list h₁
+    exact subst_concrete_expr x subsmap
+termination_by expr
+
+/--
+  Partial.Value.subst on a concrete value is that value
+-/
+theorem subst_concrete_value (value : Spec.Value) (subsmap : Map Unknown Partial.Value) :
+  (Partial.Value.value value).subst subsmap = value
+:= by
+  unfold Partial.Value.subst
+  split <;> rename_i h <;> simp only [Partial.Value.value.injEq] at h
+  subst h
+  rfl
+
+/--
+  Partial.Expr.subst on a concrete value is that value
+-/
+theorem subst_concrete_value' (value : Spec.Value) (subsmap : Map Unknown Partial.Value) :
+  value.asPartialExpr.subst subsmap = value.asPartialExpr
+:= by
+  unfold Partial.Expr.subst Spec.Value.asPartialExpr
+  cases value
+  case prim => simp only
+  case set vs =>
+    simp only [Partial.Expr.set.injEq]
+    rw [List.map₁_eq_map, List.map₁_eq_map]
+    rw [List.map_map]
+    apply List.map_congr
+    intro v _
+    exact subst_concrete_value' v subsmap
+  case record attrs =>
+    simp only [Partial.Expr.record.injEq]
+    rw [List.map_attach₂_snd]
+    rw [List.map_attach₃_snd]
+    rw [List.map_map]
+    apply List.map_congr
+    intro (k, v) _
+    simp only [Function.comp_apply, Prod.mk.injEq, true_and]
+    exact subst_concrete_value' v subsmap
+  case ext x =>
+    cases x <;> simp only [Partial.Expr.call.injEq, true_and]
+    <;> rw [List.map₁_eq_map]
+    <;> simp only [List.map_cons, List.map_nil, List.cons.injEq, and_true]
+    <;> unfold Partial.Expr.subst
+    <;> rfl
+termination_by value
+decreasing_by
+  all_goals simp_wf
+  case _ h₁ => -- set
+    have := Set.sizeOf_lt_of_mem h₁
+    omega
+  case _ h₁ => -- record
+    have h₂ := Map.sizeOf_lt_of_value h₁
+    have h₃ := Map.sizeOf_lt_of_kvs m
+    simp [Map.kvs] at h₂ h₃
+    omega
